+

src/d_find_ins_del/Post_monad.thy
@@ -1,5 +1,7 @@
 theory Post_monad imports "$SRC/c_monad/Monad" begin
 
+definition dummy :: "unit" where "dummy=Monad.dummy"
+
 (* ops types -------------------------------------------- *)
 
 datatype_record ('r,'dnode,'t) store_ops =
@@ -7,5 +9,45 @@ datatype_record ('r,'dnode,'t) store_ops =
   wrte :: "'dnode \<Rightarrow> ('r,'t) MM"
   rewrite :: "'r \<Rightarrow> 'dnode \<Rightarrow> ('r option,'t) MM"
   free :: "'r s \<Rightarrow> (unit,'t) MM"
+
+function iter_m :: "('a \<Rightarrow> ('a option,'t) MM) \<Rightarrow> 'a \<Rightarrow> ('a,'t) MM" where
+"iter_m f x = (
+  f x |> bind (% r.
+  case r of
+    None => return x
+  | Some x => iter_m f x))"
+apply (force)+ done
+termination iter_m
+ by (force intro:FIXME)
+
+
+function get_tree :: "('r,('k,'v,'r)dnode,'t) store_ops \<Rightarrow> 'r \<Rightarrow> (('k,'v)tree,'t)MM" where
+"get_tree store_ops r = (
+  r |> (store_ops|>read) |> bind (% n. case n of 
+  Disk_leaf kvs \<Rightarrow> return (Leaf(kvs))
+  | Disk_node (ks,rs) \<Rightarrow> (
+    iter_m (% (ts,rs). case rs of 
+      [] \<Rightarrow> return None
+      | r#rs \<Rightarrow> (
+        get_tree store_ops r |> bind (% t. 
+        return (Some(t#ts,rs)))))
+      ([],rs)
+    |> bind (% (ts,_).
+    return (Node(ks,List.rev ts))))))"
+apply (force)+ done
+termination get_tree
+  by (force intro:FIXME)
+
+(* check tree wellformedness from a given root *)
+definition check_tree_at_r :: "
+constants \<Rightarrow> 
+'k ord \<Rightarrow>
+('r,('k,'v,'r)dnode,'t) store_ops \<Rightarrow>
+'r \<Rightarrow> (unit,'t)MM" where
+"check_tree_at_r cs k_cmp store_ops r = (
+check_m (
+    get_tree store_ops r |> bind (% t.
+    let _ = check_true (% _. wf_tree cs None k_cmp t) in
+    return ())))"
 
 end
