src/b_pre_monad/Pre_monad.thy
@@ -6,16 +6,26 @@ Disk_node
 Key_value
 Tree
 (* Tree_stack *)
-(* don't import the states - they tend to clash with each other
+(* don't import the states - they tend to clash with each other? *)
 Find_state
 Insert_state
 Insert_many_state
 Delete_state
 Leaf_stream_state
-*)
 begin
 
-definition dummy :: "unit" where "dummy=()"
+definition dummy :: "unit" where "dummy = (
+  let _ = (% xs. (Disk_node(xs,xs) :: (int,int,int) dnode)) in
+  let _ = (% x :: (int,int,int)find_state. x) in
+  let _ = (% x :: (int,int,int)insert_state. x) in
+  let _ = (% x :: (int,int,int)delete_state. x) in
+  let _ = (% x :: (int,int,int)im_state. x) in
+  let _ = (% x :: (int,int,int)lss. x) in
+  let _ = (% x :: (int,int)tree. x) in
+  let _ = (% x :: (int + int). x) in
+  let _ = Insert_many_state.dummy in
+  ()
+)"
 
 
 end
