src/c_monad/Monad.thy
@@ -1,5 +1,6 @@
 theory Monad imports Main "$SRC/b_pre_monad/Pre_monad" begin
 
+definition dummy :: "unit" where "dummy=Pre_monad.dummy"
 
 (* abstract version; NOTE obviously can't be exported *)
 (* NOTE undefined is accepted by the code generator and allows these abstract defns to be exported *)
@@ -13,6 +14,11 @@ definition bind :: "('a \<Rightarrow> ('b,'t) MM) \<Rightarrow> ('a,'t) MM \<Rig
   
 definition return :: "'a \<Rightarrow> ('a,'t) MM" where
 "return x = undefined"
+
+(* for checking within the monad; if checking is disabled, this should just return (), else
+it should return the argument *)
+definition check_m :: "(unit,'t) MM \<Rightarrow> (unit,'t) MM" where
+"check_m x = undefined"
 
 
 end
